module TST2 where

open import Data.Nat using (ℕ; _+_; zero; suc)
import Relation.Binary.PropositionalEquality as Eq
open Eq using (_≡_; refl; cong)
open Eq.≡-Reasoning using (begin_; _≡⟨⟩_; step-≡; _∎)

+-identity : (m : ℕ) → m + zero ≡ m
+-identity zero = refl
+-identity (suc m) = cong suc (+-identity m)

+-suc : (m n : ℕ) → m + suc n ≡ suc (m + n)
+-suc zero n = refl
+-suc (suc m) n = cong suc (+-suc m n)

+-comm : (m n : ℕ) → m + n ≡ n + m
+-comm m zero = begin
    m + zero
  ≡⟨ +-identity m ⟩
    m
  ≡⟨⟩
    zero + m
  ∎
+-comm m (suc n) = begin
    m + suc n
  ≡⟨ +-suc m n ⟩
    suc (m + n)
  ≡⟨ cong suc (+-comm m n) ⟩
    suc (n + m)
  ≡⟨⟩
    suc n + m
  ∎